theories/logic/sem_sub_typing.v
@@ -30,23 +30,23 @@ Definition copy_env `{!heapGS Σ} Γ :=
 (* Sub-typing and relations *)
 
 Definition ty_le {Σ} (A B : sem_ty Σ) := ∀ v, A v ⊢ B v.
-Definition row_le {Σ} (ρ ρ' : sem_row Σ) := ⊢ iEff_le ρ ρ'.
+Definition sig_le {Σ} (ρ ρ' : sem_sig Σ) := ⊢ iEff_le ρ ρ'.
 Definition env_le `{!heapGS Σ} Γ₁ Γ₂ :=
   ∀ vs, env_sem_typed Γ₁ vs ⊢ env_sem_typed Γ₂ vs.
 
 Notation "Γ₁ '≤E' Γ₂" := (env_le Γ₁ Γ₂) (at level 98).
 Notation "τ '≤T' κ" := (ty_le τ%T κ%T) (at level 98).
 
-Notation "ρ '≤R' ρ'" := (row_le ρ%R ρ'%R) (at level 98).
+Notation "ρ '≤R' ρ'" := (sig_le ρ%R ρ'%R) (at level 98).
 
 Section sub_typing.
 
   Context `{!heapGS Σ}.
 
-  Lemma row_le_refl (ρ : sem_row Σ) : ρ ≤R ρ.
+  Lemma sig_le_refl (ρ : sem_sig Σ) : ρ ≤R ρ.
   Proof. iApply iEff_le_refl. Qed.
   
-  Lemma row_le_trans (ρ₁ ρ₂ ρ₃: sem_row Σ) : 
+  Lemma sig_le_trans (ρ₁ ρ₂ ρ₃: sem_sig Σ) : 
       ρ₁ ≤R ρ₂ →
       ρ₂ ≤R ρ₃ →
       ρ₁ ≤R ρ₃. 
@@ -55,17 +55,17 @@ Section sub_typing.
     iApply iEff_le_trans; [iApply Hρ₁₂|iApply Hρ₂₃]. 
   Qed.
   
-  Lemma row_le_bot (ρ : sem_row Σ) :
+  Lemma sig_le_nil (ρ : sem_sig Σ) :
     ⟨⟩ ≤R ρ.
   Proof. iApply iEff_le_bottom. Qed.
   
-  Lemma row_le_eff (ι₁ ι₂ κ₁ κ₂ : sem_ty Σ) :
+  Lemma sig_le_eff (ι₁ ι₂ κ₁ κ₂ : sem_ty Σ) :
     ι₁ ≤T ι₂ →
     κ₂ ≤T κ₁ →
     ((ι₁ ⇒ κ₁) ≤R (ι₂ ⇒ κ₂)).
   Proof.
     iIntros (Hι₁₂ Hκ₂₁ v) "%Φ !#".
-    rewrite !sem_row_eff_eq.
+    rewrite !sem_sig_eff_eq.
     iIntros "(%a & -> & Hι₁ & HκΦ₁)".
     iExists v. iSplit; first done. iSplitL "Hι₁".
     { by iApply Hι₁₂. }
@@ -85,44 +85,80 @@ Section sub_typing.
     iApply Hτ₂₃. by iApply Hτ₁₂.
   Qed.
   
-  Lemma ty_le_arr (τ κ : sem_ty Σ) (ρ : sem_row Σ) :
+  Lemma ty_le_u2aarr (τ κ : sem_ty Σ) (ρ : sem_sig Σ) :
     (τ -{ ρ }-> κ) ≤T (τ -{ ρ }-∘ κ).
   Proof.
-    iIntros (v) "#Hτκ %Φ %w Hw HΦ".
+    iIntros (v) "#Hτκ %w Hw".
     iApply ("Hτκ" with "Hw").
-    iIntros (u) "Hu". by iApply "HΦ".
+  Qed.
+
+  (* Lemma ty_le_u2suarr (τ κ : sem_ty Σ) (ρ : sem_sig Σ) : *)
+  (*   (τ -{ ρ }-> κ) ≤T (τ ∘-{ ρ }-> κ). *)
+  (* Proof. *)
+  (*   iIntros (v) "#Hτκ". *)
+  (*   iLöb as "IH". *)
+  (*   rewrite {2}sem_ty_equiv; [|apply sem_ty_suarr_unfold]. *)
+  (*   iIntros (w) "Hτ". *)
+  (*   assert ( *)
+  (*   iApply (ewp_mono with "[Hτκ Hτ]"). *)
+  (*   { by iApply "Hτκ". } *)
+  (*   iIntros "%u Hκ !> {$Hκ}". *)
+
+
+  Lemma ty_le_suarr2arr (τ κ : sem_ty Σ) (ρ : sem_sig Σ) :
+    (τ ∘-{ ρ }-> κ) ≤T (τ -{ ρ }-∘ κ).
+  Proof.
+    iIntros (v) "Hτκ %w Hτ".
+    rewrite sem_ty_equiv; [|apply sem_ty_suarr_unfold].
+    iApply (ewp_mono with "[Hτκ Hτ]").
+    { by iApply "Hτκ". }
+    iIntros "%u /= [Hκ _] !> {$Hκ}".
   Qed.
   
-  Lemma ty_le_larr (τ₁ κ₁ τ₂ κ₂ : sem_ty Σ) (ρ ρ' : sem_row Σ) :
+  Lemma ty_le_aarr (τ₁ κ₁ τ₂ κ₂ : sem_ty Σ) (ρ ρ' : sem_sig Σ) :
     ρ ≤R ρ' →
     τ₂ ≤T τ₁ →
     κ₁ ≤T κ₂ →
     (τ₁ -{ ρ }-∘ κ₁) ≤T (τ₂ -{ ρ' }-∘ κ₂).
   Proof.
-    iIntros (Hρ Hτ₂₁ Hκ₁₂ v) "Hτκ₁ %Φ %w Hw HΦ".
+    iIntros (Hρ Hτ₂₁ Hκ₁₂ v) "Hτκ₁ %w Hw".
     iApply ewp_os_prot_mono.
     { iApply Hρ. }
-    iApply ("Hτκ₁" with "[Hw]").
-    { by iApply Hτ₂₁. }
-    iIntros (u) "Hu". iApply "HΦ".
-    by iApply Hκ₁₂.
+    iApply (ewp_mono with "[Hτκ₁ Hw]").
+    { iApply ("Hτκ₁" with "[Hw]"); by iApply Hτ₂₁. }
+    iIntros (u) "Hu !>". by iApply Hκ₁₂.
   Qed.
   
-  Lemma ty_le_uarr (τ₁ κ₁ τ₂ κ₂ : sem_ty Σ) (ρ ρ' : sem_row Σ) :
+  Lemma ty_le_uarr (τ₁ κ₁ τ₂ κ₂ : sem_ty Σ) (ρ ρ' : sem_sig Σ) :
     ρ ≤R ρ' →
     τ₂ ≤T τ₁ →
     κ₁ ≤T κ₂ →
     (τ₁ -{ ρ }-> κ₁) ≤T (τ₂ -{ ρ' }-> κ₂).
   Proof.
-    iIntros (Hρ Hτ₂₁ Hκ₁₂ v) "#Hτκ₁ %Φ %w !# Hw HΦ".
+    iIntros (Hρ Hτ₂₁ Hκ₁₂ v) "#Hτκ₁ %w !# Hw".
     iApply ewp_os_prot_mono.
     { iApply Hρ. }
-    iApply ("Hτκ₁" with "[Hw]").
-    { by iApply Hτ₂₁. }
-    iIntros (u) "Hu". iApply "HΦ".
-    by iApply Hκ₁₂. 
+    iApply (ewp_mono with "[Hw]").
+    { iApply ("Hτκ₁" with "[Hw]"); by iApply Hτ₂₁. }
+    iIntros (u) "Hu". by iApply Hκ₁₂. 
   Qed.
   
+  Lemma ty_le_suarr (τ₁ κ₁ τ₂ κ₂ : sem_ty Σ) (ρ ρ' : sem_sig Σ) :
+    ρ ≤R ρ' →
+    τ₂ ≤T τ₁ →
+    κ₁ ≤T κ₂ →
+    (τ₁ ∘-{ ρ }-> κ₁) ≤T (τ₂ ∘-{ ρ' }-> κ₂).
+  Proof.
+    iIntros (Hρ Hτ₂₁ Hκ₁₂ v) "Hτκ₁". 
+    iLöb as "IH".
+    rewrite sem_ty_equiv; [iApply sem_ty_suarr_unfold|apply sem_ty_suarr_unfold].
+    simpl. iIntros (w) "Hτ₂". 
+    iApply (ewp_mono with "[Hτκ₁ Hτ₂]").
+    { iApply ewp_os_prot_mono. iApply Hρ. iApply "Hτκ₁". by iApply Hτ₂₁. }
+    iIntros (u) "[Hκ₁ Hτκ₁] !>". iSplitL "Hκ₁".
+    { by iApply Hκ₁₂. }
+  Admitted.
+
   Lemma ty_le_ref (τ₁ τ₂ : sem_ty Σ) :
     τ₁ ≤T τ₂ →
     (Ref τ₁) ≤T (Ref τ₂).
@@ -153,7 +189,12 @@ Section sub_typing.
     - iRight. iSplit; first done. by iApply Hκ₁₂. 
   Qed.
 
-  Lemma ty_le_forall ρ₁ ρ₂ (τ₁ τ₂ : sem_ty Σ → sem_row Σ → sem_ty Σ) :
+  Lemma ty_le_option (τ₁ τ₂ : sem_ty Σ) :
+    τ₁ ≤T τ₂ →
+    (Option τ₁) ≤T (Option τ₂).
+  Proof. intros ?. by apply ty_le_sum. Qed.
+
+  Lemma ty_le_forall ρ₁ ρ₂ (τ₁ τ₂ : sem_ty Σ → sem_sig Σ → sem_ty Σ) :
     ρ₁ ≤R ρ₂ →
     (∀ α, τ₁ α ρ₁ ≤T τ₂ α ρ₂) →
     (∀: α, ρ₁, τ₁ α ρ₁) ≤T (∀: α, ρ₂, τ₂ α ρ₂).
@@ -219,27 +260,66 @@ Section sub_typing.
     iSplitL; iExists w; by iSplit.
   Qed.
   
-  Lemma env_le_swap Γ x y τ κ :
-    (x, τ) :: (y, κ) :: Γ ≤E (y, κ) :: (x, τ) :: Γ.
-  Proof. iIntros (vs) "($ & $ & $) //=". Qed.
-  
+  Lemma env_le_bring_forth Γ n x τ :
+    nth_error Γ n = Some (x, τ) →
+    Γ ≤E (x, τ) :: (list_delete n Γ) .
+  Proof.
+    iInduction n as [|] "IH" forall (Γ); iIntros (Hnth vs).
+    { iIntros "HΓ". simpl in Hnth. destruct Γ; first done. simplify_eq. iFrame. }
+    iIntros "/= HΓ". simpl in Hnth. destruct Γ; first done; simpl. destruct p.
+    iDestruct "HΓ" as "[Hp HΓ]". iFrame. iApply "IH".
+    { by iPureIntro. }
+    iFrame.
+  Qed.
+
+  Lemma env_le_bring_forth_rev Γ n x τ :
+    nth_error Γ n = Some (x, τ) →
+    (x, τ) :: (list_delete n Γ) ≤E Γ.
+  Proof.
+    iInduction n as [|] "IH" forall (Γ); iIntros (Hnth vs).
+    { iIntros "[Hτ HΓ']". simpl in Hnth. destruct Γ; first done. simplify_eq. iFrame. }
+    iIntros "/= [Hτ HΓ]". simpl in Hnth. destruct Γ; first done; simpl. destruct p.
+    iDestruct "HΓ" as "[Hp HΓ]". iFrame. iApply "IH".
+    { by iPureIntro. }
+    iFrame.
+  Qed.
+
+  Lemma env_le_swap_second Γ x y τ₁ τ₂ : 
+    (y, τ₂) :: (x, τ₁) :: Γ ≤E (x, τ₁) :: (y, τ₂) :: Γ.
+  Proof.
+    pose proof (env_le_bring_forth_rev ((x, τ₁) :: (y, τ₂) :: Γ) 1 y τ₂).
+    by apply H.
+  Qed.
+
+  Lemma env_le_swap_third Γ x y z τ₁ τ₂ τ₃: 
+    (z, τ₃) :: (x, τ₁) :: (y, τ₂) :: Γ ≤E (x, τ₁) :: (y, τ₂) :: (z, τ₃) :: Γ.
+  Proof.
+    pose proof (env_le_bring_forth_rev ((x, τ₁) :: (y, τ₂) :: (z, τ₃) :: Γ) 2 z τ₃).
+    by apply H.
+  Qed.
+
+  Lemma env_le_weaken Γ x τ :
+    (x, τ) :: Γ ≤E Γ.
+  Proof. iIntros (vs) "(_ & $) /=". Qed.
+
 End sub_typing.
 
-Section copyable_types.
+Ltac solve_copy :=
+  repeat (intros ? ||
+          apply bi.emp_persistent ||
+          apply bi.sep_persistent ||
+          apply bi.and_persistent ||
+          apply bi.or_persistent ||
+          apply bi.forall_persistent ||
+          apply bi.exist_persistent ||
+          apply bi.pure_persistent ||
+          apply plainly_persistent ||
+          apply bi.later_persistent ||
+          apply bi.persistently_persistent ||
+          apply bi.intuitionistically_persistent ||
+          apply inv_persistent).
 
-  Ltac solve_persistent :=
-    repeat (intros ? ||
-            apply bi.sep_persistent ||
-            apply bi.and_persistent ||
-            apply bi.or_persistent ||
-            apply bi.forall_persistent ||
-            apply bi.exist_persistent ||
-            apply bi.pure_persistent ||
-            apply plainly_persistent ||
-            apply bi.later_persistent ||
-            apply bi.persistently_persistent ||
-            apply bi.intuitionistically_persistent ||
-            apply inv_persistent). 
+Section copyable_types.
   
   Context `{!heapGS Σ}.
 
@@ -248,33 +328,36 @@ Section copyable_types.
   Open Scope sem_ty_scope.
 
   Lemma copy_ty_unit : copy_ty ().
-  Proof. solve_persistent. Qed.
+  Proof. solve_copy. Qed.
   
   Lemma copy_ty_bool : copy_ty 𝔹.
-  Proof. solve_persistent. Qed.
+  Proof. solve_copy. Qed.
   
   Lemma copy_ty_nat : copy_ty ℤ.
-  Proof. solve_persistent. Qed.
+  Proof. solve_copy. Qed.
   
   Lemma copy_ty_moved : copy_ty Moved.
-  Proof. solve_persistent. Qed.
+  Proof. solve_copy. Qed.
 
   Lemma copy_ty_uarr τ ρ κ : copy_ty (τ -{ ρ }-> κ).
-  Proof. solve_persistent. Qed.
+  Proof. solve_copy. Qed.
   
   Lemma copy_ty_prod τ κ : copy_ty τ → copy_ty κ → copy_ty (τ × κ).
-  Proof. by solve_persistent. Qed.
+  Proof. by solve_copy. Qed.
   
   Lemma copy_ty_sum τ κ : copy_ty τ → copy_ty κ → copy_ty (τ + κ).
-  Proof. by solve_persistent. Qed.
+  Proof. by solve_copy. Qed.
+
+  Lemma copy_ty_option τ : copy_ty τ → copy_ty (Option τ).
+  Proof. by solve_copy. Qed.
 
   Lemma copy_ty_exists τ : (∀ α, copy_ty (τ α)) → copy_ty (∃: α, τ α).
-  Proof. solve_persistent. apply H. Qed.
+  Proof. solve_copy. apply H. Qed.
 
   Lemma copy_ty_rec τ `{NonExpansive τ}: 
     (∀ α, copy_ty (τ α)) → copy_ty (μ: α, τ α).
   Proof. iIntros (H v). rewrite sem_ty_rec_unfold.
-         solve_persistent. apply H. 
+         solve_copy. apply H. 
   Qed.
 
   Lemma copy_ty_list τ : copy_ty τ → copy_ty (List τ).
@@ -297,13 +380,13 @@ Section copyable_types.
   Qed.
 
   Lemma copy_env_nil : copy_env [].
-  Proof. solve_persistent. Qed.
+  Proof. solve_copy. Qed.
   
   Lemma copy_env_cons Γ x τ : 
     copy_env Γ →
     copy_ty τ →
     copy_env ((x, τ) :: Γ).
-  Proof. by solve_persistent. Qed.
+  Proof. by solve_copy. Qed.
 
   Lemma copy_pers τ :
     ⌜ copy_ty τ ⌝ -∗ □ (∀ v, τ v -∗ □ (τ v)).
