theories/case_studies/generator.v
@@ -1,0 +1,106 @@
+
+From iris.proofmode Require Import base tactics.
+From Coq Require Import ssreflect ssrfun ssrbool.
+
+
+(* Hazel Reasoning *)
+From program_logic Require Import weakest_precondition 
+                                  deep_handler_reasoning 
+                                  state_reasoning.
+
+(* Local imports *)
+From affine_tes.lang Require Import hazel.
+From affine_tes.logic Require Import sem_types.
+From affine_tes.logic Require Import sem_typed.
+From affine_tes.logic Require Import sem_sub_typing.
+From affine_tes.logic Require Import sem_operators.
+From affine_tes.logic Require Import compatibility.
+
+Definition generate :=
+  (λ: "i", let: "yield" := λ: "x", do: "x" in  
+           let: "cont" := ref (λ: <>, "i" "yield") in
+           λ: <>, let: "comp" := Load "cont" in 
+              TryWith ("comp" #())
+                (λ: "w" "k", ("cont" <- "k" ;; SOME "w"))%E
+                (λ: "w", "cont" <- (λ: <>,  #()) ;; NONE )%E
+  )%E. 
+
+Context `{!heapGS Σ}.
+
+Definition yield_sig (τ : sem_ty Σ) := (τ ⇒ ())%R.
+Definition yield_ty τ := τ -{ yield_sig τ }-> ().
+Definition iter_ty τ := ((yield_ty τ) -{ yield_sig τ }-∘ ())%T.
+Definition generator_ty τ := (() ∘-> Option τ)%T.
+
+Ltac solve_dom := try 
+    (apply not_elem_of_nil) || 
+    (apply not_elem_of_cons; split; solve_dom) || 
+    (intros ?; match goal with
+      | H : (BAnon ∈ env_dom _) |- _ => destruct H
+      end) ||
+    done.
+
+Ltac solve_sidecond := solve_dom; solve_copy.
+
+Lemma app_singletons {A} (x y : A) : [x;y] = [x] ++ [y].
+Proof. done. Qed.
+
+Lemma sem_typed_generate i τ :
+  ⊢ [(i, iter_ty τ)] ⊨ generate i : ⟨⟩ : generator_ty τ ⊨ [].
+Proof.
+  iIntros.
+  iApply sem_typed_app; [|iApply sem_typed_var].
+  rewrite /generate {1}(symmetry (app_nil_r [])).
+  iApply (sem_typed_afun [] [] "i" _ (iter_ty τ) ⟨⟩%R (generator_ty τ)); solve_sidecond.
+  iApply (sem_typed_let _ [("i", iter_ty τ)] _ _ _ _ (yield_ty τ)); solve_sidecond. 
+  - rewrite {1}(symmetry (app_nil_l [("i", iter_ty τ)])).
+    iApply sem_typed_ufun; solve_sidecond.
+    iApply sem_typed_do. 
+    iApply sem_typed_sub_nil.
+    iApply sem_typed_var.
+  - set cont_ty := Ref (() -{ yield_sig τ }-∘ ()). 
+    iApply (sem_typed_let _ [] _ _ _ _ cont_ty); solve_sidecond.
+    + set Γ₁ :=[("yield", yield_ty τ); ("i", iter_ty τ)].
+      iApply sem_typed_alloc.
+      rewrite -(app_nil_r Γ₁).
+      iApply sem_typed_afun; solve_dom.
+      iApply (sem_typed_app _ [("i", iter_ty τ)] _ _ _ (yield_ty τ));
+        do 2 (iApply sem_typed_sub_nil; iApply sem_typed_var).
+    + set Γ₁ :=[("cont", cont_ty)]; rewrite -(app_nil_r Γ₁). 
+      set in_cont_ty := (() -{ yield_sig τ }-∘ ()).
+      iApply sem_typed_sufun; solve_sidecond.
+      iApply (sem_typed_let _ [("cont", Ref Moved)] _ _ _ _ in_cont_ty); solve_sidecond.
+      { iApply sem_typed_sub_nil. iApply sem_typed_load. }
+      Search ( [?x; ?y] = app [?x] [?y] ).
+      rewrite app_singletons.
+      set r := fun (w : string) => ("cont" <- (λ: <>, #());; NONE)%E.
+      fold (r "w").
+      set h := fun (w k : string) => ("cont" <- "k";; SOME "w")%E.
+      fold (h "w" "k"). rewrite /yield_sig.
+      set e := ("comp" #()).
+      iPoseProof (sem_typed_shallow_try 
+                    [("comp", in_cont_ty)] [] [("cont", cont_ty)] 
+                    [("cont", Ref Moved)]
+                    "w" "k" e h r τ () (Option τ) ()) as "Hhand"; solve_sidecond.
+      rewrite /Γ₁. iApply "Hhand"; iClear "Hhand".
+      * rewrite /e. iApply sem_typed_app; iApply sem_typed_sub_nil;
+          [iApply sem_typed_var|iApply sem_typed_unit]. 
+      * rewrite /h. 
+        iApply (sem_typed_swap_third).
+        iApply sem_typed_seq.
+        { iApply sem_typed_store. 
+          iApply sem_typed_swap_third.
+          iApply sem_typed_var. }
+        iApply sem_typed_swap_second.
+        iApply sem_typed_some.
+        iApply sem_typed_var.
+      * rewrite /r. simpl.
+        iApply sem_typed_weaken.
+        iApply sem_typed_seq. 
+        iApply sem_typed_store.
+        { rewrite -(app_nil_l [("cont", Ref Moved)]). 
+          iApply (sem_typed_afun _ _ _ _ () (yield_sig τ) ()); solve_sidecond.
+          iApply sem_typed_sub_nil.
+          iApply sem_typed_unit. }
+        iApply sem_typed_none.
+Qed.
